lean/Eternity2.lean
@@ -1,4 +1,11 @@
 import Eternity2.AuxDefs
-import Eternity2.Plots
-import Eternity2.Puzzle
-
+import Eternity2.FileFormat.Puz
+import Eternity2.FileFormat.Sol
+import Eternity2.Plots.BoardSuite
+import Eternity2.Plots.GenRandom
+import Eternity2.Puzzle.Board
+import Eternity2.Puzzle.BoardSol
+import Eternity2.Puzzle.EdgeConstraints
+import Eternity2.Puzzle.SignSol
+import Eternity2.Puzzle.SolvePuzzle
+import Eternity2.Puzzle.TileSet
