lean/Eternity2/FileFormat/Puz.lean
@@ -1,0 +1,96 @@
+import Eternity2.Puzzle.TileSet
+
+namespace Eternity2.FileFormat.TileSet
+
+def toFileFormat.color (c : Color.WithBorder s) : String :=
+  match c with
+  | .frame => "0"
+  | .border n _ | .center n _ => toString n
+
+def toFileFormat.tile (t : Tile (Color.WithBorder s)) : String :=
+  s!"{color t.up} {color t.right} {color t.down} {color t.left}{
+      match t.sign with
+      | none => ""
+      | some .plus => " +"
+      | some .minus => " -"
+    }"
+
+def toFileFormat (ts : TileSet size (Tile (Color.WithBorder s))) :=
+  s!"{size} {size}\n" ++
+  String.intercalate "\n"
+    ( ts.tiles.map toFileFormat.tile ) ++ "\n"
+
+def ofFileFormat (s : String) :
+  Except String (Σ size s, TileSet size (Tile (Color.WithBorder s)))
+  := do
+  match s.splitOn "\n"
+    |>.filter (fun line => !line.startsWith "c" && !line.isEmpty)
+  with
+  | [] => throw "No board size line in file"
+  | sline::rest =>
+  let size ←
+    match sline.splitOn " " with
+    | [w] => pure <| String.toNat! w
+    | [w, h] =>
+      if w = h then
+        pure <| String.toNat! w
+      else throw "Not a square (currently unsupported)"
+    | _ => throw s!"Expected board size line `<cols> [rows]`, but got: {sline}"
+
+  let tiles : List (Tile Nat) ←
+    rest
+    |>.filter (!·.all Char.isWhitespace)
+    |>.mapM (fun s => do
+      match s.splitOn " " with
+      | up :: right :: down :: left :: rest =>
+        let parse := (fun s => s.toNat? |>.expectSome fun () => s!"expected nat, got {s}")
+        let (up, right, down, left) :=
+          (← parse up, ← parse right, ← parse down, ← parse left)
+        return { up, right, down, left, sign := ← (do match rest with
+          | ["+"] => return some .plus
+          | ["-"] => return some .minus
+          | []    => return none
+          | _ => throw s!"Expected end-of-line, got {String.intercalate " " rest}"
+          )}
+      | _ =>
+        throw s!"Bad input line: \"{s}\"")
+  
+  if tiles.all (·.colors.all (· > 0)) then
+    throw "Appears to be an unframed puzzle; these are not yet supported."
+
+  let (borderColors, centerColors) ←
+    tiles.foldlM (fun (bc,cc) y => do
+      match y.classifyGen 0 with
+      | none => throw s!"Piece has an invalid shape: {y}"
+      | some ⟨_, .corner x y _⟩ => return (x::y::bc, cc)
+      | some ⟨_, .side x y z _⟩ => return (x::z::bc, y::cc)
+      | some ⟨_, .center w x y z _⟩ => return (bc, w::x::y::z::cc))
+    ([],[])
+
+  let borderColors := borderColors.distinct
+  let centerColors := centerColors.distinct
+
+  let s : Color.WithBorder.Settings := ⟨borderColors,centerColors⟩
+
+  let tileMap (t : Tile Nat) : Except String (Tile (Color.WithBorder s)) := do
+    match t.classifyGen 0 with
+    | none => throw "misclassified even though should have errored earlier? 5467654"
+    | some ⟨n, .corner x y _⟩ =>
+      return {  up   := .border x sorry , right := .border y sorry
+             ,  down := .frame          , left  := .frame         , sign := t.sign }
+    | some ⟨n, .side x y z _⟩ =>
+      return {  up   := .border x sorry , right := .center y sorry
+             ,  down := .border z sorry , left  := .frame         , sign := t.sign }
+    | some ⟨n, .center w x y z _⟩ =>
+      return {  up   := .center w sorry , right := .center x sorry
+             ,  down := .center y sorry , left  := .center z sorry, sign := t.sign }
+
+
+  let tiles ← tiles.mapM (tileMap)
+  if h : tiles.length = size * size then
+    return ⟨size, s, tiles, h⟩
+  else
+    throw s!"File lists {tiles.length} pieces, but {size*size} were expected"
+
+
+def ofFile (f : System.FilePath) := IO.FS.withFile f .read (·.readToEnd) >>= IO.ofExcept ∘ ofFileFormat
