lean/Eternity2/FileFormat/Sol.lean
@@ -1,0 +1,61 @@
+import Eternity2.Puzzle.BoardSol
+
+namespace Eternity2.FileFormat.BoardSol
+
+def toFile (filename : System.FilePath)
+    [BEq c] {ts : TileSet size c} (sol : BoardSol ts)
+                : IO Unit := do
+  IO.FS.withFile filename .write (fun h => do
+    h.putStrLn "c pieceNum x y rotation"
+    h.putStrLn ""
+    for i in List.fins _ do
+      let (⟨x,y⟩,rot) := sol.pieceIdx i
+      h.putStrLn s!"{i} {x} {y} {rot}"
+  )
+
+def ofFileFormat (contents : String)
+                 (ts : TileSet size (Tile <| Color.WithBorder s))
+               : Except String (BoardSol ts) := do
+  let data ← do
+    let lines :=
+      contents.splitOn "\n"
+      |>.map (·.trim) |>.filter (fun l => !(l.length = 0 || l.startsWith "c"))
+    let parsed ← lines.mapM parseLine 
+    pure <| parsed.foldl (init := Std.HashMap.empty) (fun map (t,loc) => map.insert t loc)
+
+  let array ← Array.initM (size*size) (fun i => do
+      match data.find? i with
+      | none => throw s!"Piece {i} is missing from solution"
+      | some (x,y,r) => pure (⟨x,y⟩,r))
+  have : array.size = size*size := sorry
+  return ⟨(array[this.symm ▸ ·])⟩
+
+where parseLine : String → Except String (Fin _ × Fin _ × Fin _ × Fin 4) := fun line => do
+    match line.splitOn " " with
+    | [t, x, y, r] => (
+      match (t.toNat?, x.toNat?, y.toNat?, r.toNat?) with
+      | (some t, some x, some y, some r) =>
+        if ht : t ≥ size*size then
+          throw s!"Tile index out of range: {line}"
+        else if hx : x ≥ size then
+          throw s!"Row {x} out of range: {line}"
+        else if hy : y ≥ size then
+          throw s!"Col {y} out of range: {line}"
+        else if hr : r ≥ 4 then
+          throw s!"Rotation {r} out of range: {line}"
+        else
+        return (
+          ⟨t,Nat.not_ge_eq _ _ ▸ ht⟩,
+          ⟨x,Nat.not_ge_eq _ _ ▸ hx⟩,
+          ⟨y,Nat.not_ge_eq _ _ ▸ hy⟩,
+          ⟨r, by rw [Nat.not_ge_eq] at hr; exact hr⟩)
+      | _ => throw s!"Could not parse integers on line: {line}"
+    )
+    | _ => throw s!"Incorrectly formatted sol line: {line}"
+
+def ofFile (ts : TileSet size (Tile <| Color.WithBorder s)) (filename : System.FilePath) :=
+  show IO _ from do
+  let contents ← IO.FS.withFile filename .read (fun handle =>
+    handle.readToEnd
+  )
+  return ← IO.ofExcept <| ofFileFormat contents ts
