lean/Eternity2/Plots/BoardSuite.lean
@@ -1,0 +1,38 @@
+import Eternity2.Puzzle.BoardSol
+import Eternity2.FileFormat.Puz
+import Eternity2.FileFormat.Sol
+
+open System
+
+namespace Eternity2
+
+structure SolvedBoard where
+  size : Nat
+  colors : Color.WithBorder.Settings
+  tiles : TileSet size (Tile <| Color.WithBorder colors)
+  sols : Array (BoardSol tiles)
+  allSols : Bool
+
+structure BoardSuite where
+  boards : Array SolvedBoard
+
+def BoardSuite.ofDirectory (path : FilePath) : IO BoardSuite := do
+
+  -- find all .puz files in the directory
+  let puzFiles ← path.walkDir (fun p => do return p.extension = some "puz")
+
+  let boards ← puzFiles.mapM (fun file => do
+    -- read the .puz file
+    let ⟨size, colors, ts⟩ ← FileFormat.TileSet.ofFile file
+    
+    -- get all the .sol files in the same directory
+    let solFiles ← (file.withFileName ".").walkDir (fun p => do return p.extension = some "sol")
+
+    -- read each .sol file as a solution to `ts`
+    let sols ← solFiles.mapM (FileFormat.BoardSol.ofFile ts)
+
+    -- check whether `done` file is present in directory (which indicates all solutions were found)
+    let done ← (file.withFileName "done").pathExists
+
+    return ⟨size,colors,ts,sols,done⟩)
+  return ⟨boards⟩
