lean/Eternity2/Puzzle.lean
@@ -1,6 +1,0 @@
-import Eternity2.Puzzle.Board
-import Eternity2.Puzzle.EdgeConstraints
-import Eternity2.Puzzle.GenBoard
-import Eternity2.Puzzle.SolvePuzzle
-import Eternity2.Puzzle.TileSet
-import Eternity2.Puzzle.SignSol
