lean/Eternity2/Puzzle/BoardSol.lean
@@ -1,0 +1,72 @@
+import Eternity2.Puzzle.Board
+import Eternity2.Puzzle.TileSet
+import Eternity2.Puzzle.EdgeConstraints
+
+namespace Eternity2
+
+structure BoardSol [BEq c] (ts : TileSet size c) where
+  /-- For each tile in tileset, its index + rotation (0 = up) -/
+  pieceIdx : Fin (size * size) → SquareIndex size × Fin 4
+
+namespace BoardSol
+
+def toTileBoard {ts : TileSet size (Tile <| Color.WithBorder s)}
+                          (sol : BoardSol ts)
+    : IO (TileBoard size (Color.WithBorder s)) := do
+  let mut temp_board :=
+    Array.init size (fun _ => Array.init size (fun _ => none))
+  for t in List.fins _ do
+    let (⟨x,y⟩,r) := sol.pieceIdx t
+    temp_board :=
+      temp_board.set! y (temp_board[y]!.set! x (some <| ts.tiles[ts.h_ts.symm ▸ t].rotln r))
+
+  let board := Array.init size (fun y =>
+    Array.init size (fun x =>
+      match temp_board[y]![x]! with
+      | some t => t
+      | none => panic! "Incomplete solution loaded"
+    )
+  )
+
+  let tb : TileBoard size (Color.WithBorder s) := {
+    board := board
+    board_size := by simp
+  }
+  return tb
+
+def ofTileBoard (tb : TileBoard size (Color.WithBorder s))
+  : Σ ts : TileSet size (Tile <| Color.WithBorder s), BoardSol ts :=
+  let withIdx : Array (SquareIndex size × Tile _) :=
+    (Array.init size fun i => Array.init size fun j =>
+      (⟨i,j⟩,tb.board[tb.board_size.1.symm ▸ i][(tb.board_size.2 _ _).symm ▸ j])
+    ).flatten
+  have : withIdx.size = size*size := sorry
+  ⟨ ⟨withIdx.map (·.2) |>.toList, sorry⟩
+  , ⟨fun idx => (withIdx[this.symm ▸ idx].1, 0)⟩
+  ⟩
+
+/- Randomly rotate the tiles, and mix up their order -/
+def scramble {ts : TileSet size (Tile <| Color.WithBorder s)} (sol : BoardSol ts)
+  : IO ((ts : TileSet size (Tile <| Color.WithBorder s)) × BoardSol ts) := do
+  /- Rotate the pieces -/
+  let rotated ← ts.tiles.enum'.mapM (fun (i, tile) => do
+    let rot ← IO.rand 0 3
+    let rot' : Fin 4 := ⟨rot, sorry⟩
+    /- og index, rotation vs og, rotated tile -/ 
+    return (ts.h_ts ▸ i, rot', tile.rotln rot'))
+  /- Randomly permute the corners/sides/centers -/
+  let corners ← rotated.filter (·.2.2.isCorner) |> IO.randPerm
+  let sides   ← rotated.filter (·.2.2.isSide)   |> IO.randPerm
+  let centers ← rotated.filter (·.2.2.isCenter) |> IO.randPerm
+  /- Recombine -/
+  have all := corners.toArray ++ sides ++ centers
+  have h_all : all.size = size * size := sorry
+  /- Tileset -/
+  let tiles := all.toList.map (·.2.2)
+  have h_tiles : tiles.length = size * size := by simp [h_all]
+  /- solution -/
+  let sol := Array.init (size*size) (fun i =>
+    let (old_i, rot, tile) := all[h_all.symm ▸ i]
+    let (pos, old_rot) := sol.pieceIdx old_i
+    (pos,rot+old_rot))
+  return ⟨⟨tiles, h_tiles⟩, ⟨(sol[·])⟩⟩
