lean/Eternity2/Puzzle/TileSet.lean
@@ -4,108 +4,24 @@ namespace Eternity2
 
 open Std
 
-structure TileSet (size : Nat) (color : Type u) [BEq color] where
-  tiles : List (Tile color)
+structure TileSet (size : Nat) (tile : Type u) where
+  tiles : List (tile)
   h_ts : tiles.length = size * size
 
-instance [BEq c] : BEq (TileSet s c) := ⟨(·.tiles == ·.tiles)⟩
+instance [BEq t] : BEq (TileSet s t) := ⟨(·.tiles == ·.tiles)⟩
 
 namespace TileSet
 
-instance [BEq color] [Inhabited color] : Inhabited (TileSet size color) where
+instance [Inhabited tile] : Inhabited (TileSet size tile) where
   default := {
     tiles := List.replicate (size * size) default
     h_ts := by simp
   }
 
-def toFileFormat (ts : TileSet size (Color.withBorder b c)) : String :=
-  s!"c {size}x{size} board with {b} border colors, {c} center colors\n" ++
-  s!"p tile {size} {size}\n" ++
-  String.intercalate "\n"
-    ( ts.tiles.map (fun {up, right, down, left} =>
-        s!"{up.val} {right.val} {down.val} {left.val}"
-      )
-    ) ++ "\n"
-
-
-def toFile (file : System.FilePath) (ts : TileSet size (Color.withBorder b c)) : IO Unit := do
-  IO.FS.withFile file .write (fun handle =>
-    handle.putStr (toFileFormat ts))
-
-def fromFile (file : System.FilePath) : IO (Σ size b c, TileSet size (Color.withBorder b c)) := do
-  let contents ← IO.FS.withFile file .read (fun handle =>
-    handle.readToEnd
-  )
-  match contents.splitOn "\n"
-    |>.filter (!·.startsWith "c")
-    |>.dropWhile (fun s => !s.startsWith "p")
-  with
-  | [] => panic! "No p line in file"
-  | pline::rest =>
-  let size :=
-    match pline.splitOn " " with
-    | ["p", "tile", w] => String.toNat! w
-    | ["p", "tile", w, h] =>
-      if w = h then String.toNat! w else panic! "Not a square (currently unsupported)"
-    | ["p", "tile", w, h, _] =>
-      if w = h then String.toNat! w else panic! "Not a square (currently unsupported)"
-    | _ => panic! s!"Incorrectly formatted p line: {pline}"
-
-  let tiles : List (Tile Nat)
-    ← rest
-    |>.filter (!·.all Char.isWhitespace)
-    |>.mapM (fun s =>
-      match s.splitOn " " |>.map String.toNat? with
-      | [some up, some right, some down, some left] =>
-        return { up, right, down, left }
-      | _ =>
-        panic! s!"Bad input line: \"{s}\"")
-  
-  let maxCenterColor := tiles.map (fun t =>
-      t.colors.maximum?.getD 0
-    )
-    |>.maximum?.getD 0
-
-  let b := tiles.map (fun t =>
-      (if t.up    = 0 then [t.left, t.right] else []) ++
-      (if t.right = 0 then [t.up  , t.down ] else []) ++
-      (if t.down  = 0 then [t.left, t.right] else []) ++
-      (if t.left  = 0 then [t.up  , t.down ] else [])
-      |>.maximum?.getD 0
-    )
-    |>.maximum?.getD 0
-
-  let c := maxCenterColor - b
-
-  let cMap (i : Nat) : IO (Color.withBorder b c) :=
-    if _ : i = 0 then
-      return Color.frameColor
-    else if _ : i ≤ b then
-      return Color.borderColor ⟨i-1,
-        Nat.lt_of_lt_of_le (Nat.pred_lt (by assumption)) (by assumption)⟩
-    else if _ : i ≤ maxCenterColor then
-      assert! i-b-1 < c
-      return Color.centerColor ⟨i-b-1,
-        by sorry⟩
-    else
-      panic! s!"Found color {i}, even though maxCenterColor={maxCenterColor}"
-
-  let tiles ← tiles.mapM (fun t => do
-    let t : Tile _ := { up := ← cMap t.up, right := ← cMap t.right, down := ← cMap t.down, left := ← cMap t.left }
-    if t.validate then
-      return t
-    else
-      panic! s!"Interpreting file as having {b} border colors, {c} center colors, found invalid piece:\n{t}"
-  )
-  if h : tiles.length = size * size then
-    return ⟨size, b, c, ⟨tiles, h⟩⟩
-  else
-    panic! s!"File lists {tiles.length} pieces, but {size*size} were expected"
-
-def toString (ts : TileSet size (Color.withBorder b c)) : String :=
-  ts.tiles.map (·.toString)
+nonrec def toString [ToString tile] (ts : TileSet size tile) : String :=
+  ts.tiles.map (toString ·)
   |>.map (·.splitOn "\n")
   |>.foldl (fun L1 L2 => List.zipWith (· ++ " " ++ ·) L1 L2) ["","",""]
   |> String.intercalate "\n"
 
-instance : ToString (TileSet size (Color.withBorder b c)) := ⟨toString⟩
+instance [ToString tile] : ToString (TileSet size tile) := ⟨toString⟩
